Strata/Languages/Core/Identifiers.lean
@@ -56,7 +56,13 @@ instance : Inhabited CoreIdent where
 
 instance : Lambda.HasGen Unit where
   genVar T := let (sym, state') := (Lambda.TState.genExprSym T.genState)
-              (⟨sym, ()⟩, { T with genState := state' })
+              .ok (⟨sym, ()⟩, { T with genState := state' })
+  genVar_tyGen_mono := by
+    intro Env xv Env' h
+    simp at h
+    obtain ⟨_, h_env⟩ := h
+    rw [← h_env]
+    simp [Lambda.TState.genExprSym, Lambda.TState.incExprGen]
 
 namespace Syntax
 
